src/assembly.lean
@@ -1,0 +1,38 @@
+import tactic.tidy
+
+-- assembly verification
+
+inductive assembly.expr
+| cons : ℕ → assembly.expr
+| register : fin 12 → assembly.expr
+
+inductive assembly.cmd
+| mov : assembly.expr → assembly.expr → assembly.cmd
+| add : assembly.expr → assembly.expr → assembly.cmd
+
+def assembly.program := list assembly.cmd
+
+def assembly.state := fin 12 → ℕ
+
+-- def assembly.run (state : assembly.state) :
+--                   assembly.cmd → option assembly.state
+-- | (cmd.mov (expr.cons n) (expr.register i)) := some $ λ r,
+--                                                if r = i 
+--                                                then n
+--                                                else state r
+-- | (cmd.mov (expr.register j) (expr.register i)) := some $ λ r,
+--                                                    if r = i
+--                                                    then state j
+--                                                    else state r
+-- | (cmd.add a a_1) := sorry
+-- | _  := none
+
+example : ∀ n : ℕ, ∃ m : ℕ, n + 1 = m  :=
+begin
+    intro n,
+    existsi n+1,
+    refl,
+end
+
+
+
