src/enderton_predicate_logic.lean
@@ -1,0 +1,663 @@
+import data.set.countable tactic.find tactic.tidy tactic.ring
+universe u
+
+-- We introduce a much simplified version of
+-- untyped first order (minimal) predicate logic.
+
+-- make all propositions decidable. 
+-- Allows us to freely use ifs like in Haskell
+-- but then we must add noncomputable to all functions
+-- local attribute [instance] classical.prop_decidable
+
+
+namespace logic
+
+open logic list tactic set
+
+section formulas
+parameters {functional_symbol : Type u} [decidable_eq functional_symbol]
+parameter {relational_symbol : Type u}
+parameter {arity : functional_symbol -> ℕ}
+parameter {rarity : relational_symbol -> ℕ}
+
+-- arity types
+def is_constant (f : functional_symbol) := arity f = 0
+def nary (n : ℕ) := subtype {f : functional_symbol | arity f = n}
+def nrary (n : ℕ) := subtype {r : relational_symbol | rarity r = n}
+@[reducible]
+def const := nary 0
+
+-- terms in the language
+inductive term
+| var : ℕ → term
+| app  {n : ℕ} (f : nary n) (v : fin n → term) :  term
+
+-- constant terms.
+def const.term : const → term
+| c := term.app c fin_zero_elim
+
+@[reducible]
+def term.rw : term → ℕ → term → term
+| (term.var a) x t := if x = a then t else term.var a
+| (term.app f v) x t := 
+    let v₂ := λ m, term.rw (v m) x t in
+    term.app f v₂
+
+def term.vars : term → list ℕ
+| (term.var a) := [a]
+| (term.app  f v) :=
+    let v₂ := λ m, term.vars (v m) in
+    foldr (++) [] (of_fn v₂)
+
+@[reducible]
+def term.denotes (t : term) := t.vars = []
+@[reducible]
+def term.conotes (t : term) := ¬ t.denotes
+
+-- a term in the proper sense of the term (pun intended).
+def pterm := subtype {t : term | t.denotes}
+def expression := subtype {t : term | t.conotes}
+
+-- def term.subterms : term → set term
+-- | (term.app f v) := 
+--     let v₂ := λ m, term.subterms (v m) in
+--     (⋃ m, v₂ m) ∪ {(term.app f v)}
+-- | t := {t}
+
+def list.vars : list term → list ℕ
+| [] := ∅
+| (hd :: tl) := hd.vars ++ tl.vars
+
+-- def list.subterms : list term → list term
+-- | [] := ∅
+-- | (hd :: tl) := hd.subterms ++ tl.subterms
+
+def list.rw : list term → ℕ → term → list term
+| [] _ _:= ∅
+| (hd :: tl) x t := (hd.rw x t) :: tl.rw x t
+
+-- def subterms : set term → list term
+-- | S := ⋃ x ∈ S, term.subterms x
+
+-- formulas
+inductive uformula
+| relational {n : ℕ} (r : nrary n) (v : fin n → term) : uformula
+| equation (t₁ t₂ : term) : uformula
+| false : uformula
+| for_all :  ℕ → uformula → uformula
+| if_then : uformula → uformula → uformula
+
+def uformula.not (φ) := uformula.if_then φ uformula.false
+
+reserve infixr ` ⇒ `:55
+class has_exp (α : Type u) := (exp : α → α → α)
+infixr ⇒ := has_exp.exp
+instance uformula.has_exp : has_exp uformula := ⟨uformula.if_then⟩
+
+local notation `∼` := uformula.not
+
+@[reducible]
+def uformula.rw : uformula → ℕ → term → uformula
+| (uformula.relational r v) x t :=
+    let v₂ := λ m, (v m).rw x t in
+    uformula.relational r v₂
+| (uformula.equation t₁ t₂) x t :=
+    let t₃ := t₁.rw x t,
+        t₄ := t₂.rw x t
+    in uformula.equation t₃ t₄
+| (uformula.for_all y φ) x t :=
+    let ψ := if y = x then φ else φ.rw x t in
+    uformula.for_all y ψ
+| (uformula.if_then φ ψ) x t := uformula.if_then (φ.rw x t) (ψ.rw x t)
+| φ _ _ := φ
+
+def list_sub_aux {α} [decidable_eq α] : list α → list α → list α
+| [] _ := []
+| (hd::tl) xs := 
+begin
+    cases list.decidable_mem hd xs,
+        exact hd :: list_sub_aux tl xs,
+    exact list_sub_aux tl xs,
+end
+                
+instance list_sub {α} [decidable_eq α] : has_sub (list α) :=
+⟨list_sub_aux⟩
+
+-- free variables
+@[reducible]
+def uformula.free : uformula → list ℕ
+| (uformula.relational r v) := list.vars (of_fn v)
+| (uformula.equation t₁ t₂) := t₁.vars ++ t₂.vars
+| (uformula.for_all x φ) := φ.free - [x]
+| (uformula.if_then φ ψ) := φ.free ++ ψ.free
+| _ := []
+
+-- open and closed formulas.
+def uformula.closed : uformula → Prop
+| φ := φ.free = ∅
+
+def uformula.open : uformula → Prop
+| φ := ¬ φ.closed
+
+def uformula.vars : uformula → list ℕ
+| (uformula.for_all x φ) := x::φ.free
+| (uformula.if_then φ ψ) := φ.vars ++ ψ.vars
+| φ := φ.free
+
+inductive uaxiom : uformula → Prop
+| p₁ (φ ψ : uformula) : uaxiom (φ ⇒ ψ ⇒ φ)
+| p₂ (φ ψ δ : uformula) : uaxiom ((φ ⇒ ψ ⇒ δ) ⇒ ((φ ⇒ ψ) ⇒ φ ⇒ δ))
+| p₃ (φ ψ : uformula) : uaxiom ((∼φ ⇒ ∼ψ) ⇒ ψ ⇒ φ)
+| q₅ (x : ℕ) (φ : uformula) (t : pterm) : uaxiom ((uformula.for_all x φ) ⇒ φ.rw x t.val)
+| q₆ (x : ℕ) (φ ψ : uformula) : uaxiom ((uformula.for_all x φ ⇒ ψ) ⇒ (uformula.for_all x φ) ⇒ (uformula.for_all x ψ))
+| q₇ (x : ℕ) (φ : uformula) (x ∉ φ.free) : uaxiom (φ ⇒ (uformula.for_all x φ))
+
+inductive argument
+| silence {} : argument -- empty argument
+| node : uformula → argument → argument → argument → argument
+
+def argument.assumes (φ : uformula) : argument → Prop
+| argument.silence := false
+| (argument.node ψ argument.silence argument.silence argument.silence) := φ = ψ
+| (argument.node _ a₁ a₂ a₃) := a₁.assumes ∨ 
+                                a₂.assumes ∨ 
+                                a₃.assumes
+
+@[reducible]
+def argument.concludes (φ : uformula) : argument → Prop
+| argument.silence := false
+| (logic.argument.node ψ x y z) := ψ = φ
+
+-- def silence := argument.silence
+-- -- because I said so
+-- def argument.return : uformula → argument
+-- | φ := argument.node φ silence silence silence
+
+-- tells whether an argument is a proof from Γ
+-- TODO: CONVERT THIS TO INDUCTIVE DEFINITION !!!!
+@[reducible]
+def argument.proof_from (Γ : set uformula) : argument → Prop
+| (argument.node φ argument.silence argument.silence argument.silence) := φ ∈ Γ ∨
+                                                                          φ = uformula.true ∨
+                                                                          ∃ t, φ = uformula.equation t t
+-- introduction rules
+| (argument.node (uformula.and φ ψ)
+                       γ₁
+                       γ₂
+                       argument.silence) := γ₁.concludes φ ∧
+                                            γ₂.concludes ψ ∧
+                                            γ₁.proof_from ∧
+                                            γ₂.proof_from
+| (argument.node (uformula.or φ _)
+                       γ₁
+                       argument.silence
+                       argument.silence) := γ₁.concludes φ ∧ γ₁.proof_from
+| (argument.node (uformula.or _ ψ)
+                       argument.silence
+                       γ₂
+                       argument.silence) := γ₂.concludes ψ ∧ γ₂.proof_from
+| (argument.node (uformula.if_then φ ψ)
+                       γ
+                       argument.silence
+                       argument.silence) := γ.concludes ψ ∧
+                                            γ.assumes φ ∧
+                                            γ.proof_from
+| (argument.node (uformula.for_all x φ)
+                       γ
+                       argument.silence
+                       argument.silence) := ∃ c, γ.concludes (φ.rw x $ term.abs c) ∧
+                                            x ∈ φ.free ∧
+                                            γ.proof_from
+| (argument.node (uformula.exist x φ)
+                       γ
+                       argument.silence
+                       argument.silence) := ∃ t, γ.concludes (φ.rw x t) ∧
+                                            t.denotes ∧
+                                            x ∈ φ.free ∧
+                                            γ.proof_from
+-- elimination rules
+| (argument.node φ γ argument.silence argument.silence) := ((∃ ψ, γ.concludes $ uformula.and φ ψ) ∨
+                                                            (∃ ψ, γ.concludes $ uformula.and ψ φ) ∨
+                                                            (∃ x (ψ : uformula) (t : term), 
+                                                             t.denotes ∧
+                                                             x ∈ ψ.free ∧
+                                                             γ.concludes (uformula.for_all x ψ) ∧
+                                                             φ = ψ.rw x t)) ∧
+                                                             γ.proof_from
+| (argument.node φ γ₁ γ₂ argument.silence) := ((∃ ψ, γ₁.concludes (ψ ⇒ φ) ∧
+                                               γ₂.concludes ψ) ∨
+                                              (∃ x (ψ : uformula) c,
+                                               x ∈ ψ.free ∧
+                                               γ₁.concludes (uformula.exist x ψ) ∧
+                                               γ₂.concludes ((ψ.rw x $ term.abs c) ⇒ φ)) ∨
+                                              (∃ x (ψ : uformula) (t₁ t₂ : term), 
+                                               t₁.denotes ∧
+                                               t₂.denotes ∧
+                                               x ∈ ψ.free ∧
+                                               γ₁.concludes (ψ.rw x t₁) ∧
+                                               γ₂.concludes (uformula.equation t₁ t₂) ∧
+                                               φ = ψ.rw x t₂)) ∧
+                                               γ₁.proof_from ∧
+                                               γ₂.proof_from
+| (argument.node φ γ₁ γ₂ γ₃) := ∃ ψ₁ ψ₂, γ₁.concludes (uformula.or ψ₁ ψ₂) ∧
+                                         γ₂.concludes (ψ₁ ⇒ φ) ∧
+                                         γ₃.concludes (ψ₂ ⇒ φ) ∧
+                                         γ₁.proof_from ∧
+                                         γ₂.proof_from ∧
+                                         γ₃.proof_from
+| _ := false
+
+
+def argument.proof_of (φ : uformula) (Γ : set uformula) : argument → Prop
+| γ := γ.proof_from Γ ∧ γ.concludes φ 
+
+variables (Γ : set uformula) (φ : uformula)
+
+theorem self_entailment : minimal.entails Γ (φ ⇒ φ) :=
+begin
+    apply minimal.entails.intro,
+    apply minimal.entails.reflexive (Γ∪{φ}) φ,
+    simp
+end
+
+theorem id_symm : ∀ (t₁ t₂ : pterm),
+                  minimal.entails Γ (uformula.equation t₁.val t₂.val) →
+                  minimal.entails Γ (uformula.equation t₂.val t₁.val)  :=
+let ne := var_ne in
+begin
+    intros t₁ t₂ h,
+    apply nonempty.elim ne, intro x,
+    -- φ := "x = t₁"
+    let φ := uformula.equation (term.var x) t₁.val,
+    have den₁ := t₁.property.1,
+    have den₂ := t₂.property.1,
+    have c₀ : x ∈ φ.free, simp[φ],
+    have c₁ : minimal.entails Γ (φ.rw x t₁.val),
+        simp[φ],
+        dunfold uformula.rw, simp,
+        dunfold term.rw, simp,
+        rw den_rw t₁.val t₁.val x t₁.property.1,
+        apply minimal.entails.identity_intro Γ t₁.val,
+    have c₂ : minimal.entails Γ (φ.rw x t₂.val),
+        apply minimal.entails.identity_elim, --Γ φ x c₀ t₁ t₂ den₂ den₁,
+        repeat {assumption <|> apply_assumption},
+    simp[φ] at c₂,
+    have c₃ : (uformula.equation (term.var x) (t₁.val)).rw x (t₂.val) = uformula.equation (t₂.val) (t₁.val),
+        dunfold uformula.rw, simp,
+        constructor,
+            dunfold term.rw, simp,
+        apply den_rw t₁.val t₂.val x den₁,
+    rwa c₃ at c₂,
+end
+
+variables (Δ : set uformula) (ψ : uformula)
+
+theorem monotonicity : Δ ⊆ Γ → minimal.entails Δ ψ → minimal.entails Γ ψ :=
+begin
+    intros H h,
+    -- induction on the possible ways in which
+    -- Δ could prove ψ
+    induction h,
+    -- case it was proven by reflection
+        apply minimal.entails.reflexive Γ h_φ,
+        exact H h_h,
+    -- case it was proven by transitivity
+        apply minimal.entails.transitivity Γ h_Δ h_φ,
+        intros ψ₂ elem,
+        repeat {assumption <|> apply_assumption},
+    -- case it was proven by and_intro
+        apply minimal.entails.and_intro,-- h_φ h_ψ Γ,
+        repeat {assumption <|> apply_assumption},
+    -- case it was proven by and_elim_left
+        apply minimal.entails.and_elim_left h_φ h_ψ Γ,
+        repeat {assumption <|> apply_assumption},
+    -- case it was proven by and_elim_right
+        apply minimal.entails.and_elim_right h_φ h_ψ Γ,
+        repeat {assumption <|> apply_assumption},
+    -- case it was proven by or_intro_left
+        apply minimal.entails.or_intro_left h_φ h_ψ Γ,
+        repeat {assumption <|> apply_assumption},
+    -- case it was proven by or_intro_right
+        apply minimal.entails.or_intro_right h_φ h_ψ Γ,
+        repeat {assumption <|> apply_assumption},
+    -- case it was proven by or_elim
+        apply minimal.entails.or_elim,-- h_φ h_ψ h_δ Γ,
+        repeat {assumption <|> apply_assumption},
+    -- case it was proven by modus ponens
+        apply minimal.entails.modus_ponens h_φ h_ψ Γ,
+        repeat {assumption <|> apply_assumption},
+    -- case it was proven by intro
+        have c : minimal.entails h_Γ (h_φ ⇒ h_ψ),
+            apply minimal.entails.intro h_φ h_ψ h_Γ,
+            assumption,
+        apply minimal.entails.transitivity Γ h_Γ (h_φ ⇒ h_ψ),
+            intros ψ₂ elem,
+            have c₂ := H elem,
+            exact minimal.entails.reflexive Γ ψ₂ c₂,
+        assumption,
+    -- case it was proven by true_intro
+        exact minimal.entails.true_intro Γ,
+    -- case it was proven by for_all_intro
+        apply minimal.entails.for_all_intro Γ h_φ h_x h_xf h_c,
+        repeat {assumption <|> apply_assumption},
+    -- case it was proven by for_all_elim
+        apply minimal.entails.for_all_elim Γ h_φ h_x h_xf,
+        repeat {assumption <|> apply_assumption},
+    -- case it was proven by exists_intro
+        apply minimal.entails.exists_intro Γ h_φ h_x h_xf h_t,
+        repeat {assumption <|> apply_assumption},
+    -- case it was proven by exists_elim
+        apply minimal.entails.exists_elim Γ h_φ h_ψ h_x h_xf,
+        repeat {assumption <|> apply_assumption},
+    -- case it was proven by identity_intro
+        apply minimal.entails.identity_intro Γ h_t,
+    -- case it was proven by identity_elim
+        apply minimal.entails.identity_elim Γ h_φ h_x h_xf h_t₁ h_t₂,
+        repeat {assumption <|> apply_assumption},
+end
+
+
+theorem proof_entails : (∃ p : argument, p.proof_of φ Γ) → minimal.entails Γ φ :=
+begin
+    intro h,
+    obtain ⟨p, ph₁, ph₂⟩ := h,
+    induction p,
+        have c : false := ph₂,
+        contradiction,
+    have eq : φ = p_a := sorry, 
+        -- impossible to unfold at ph₂ for some reason
+        -- simp [argument.concludes] at ph₂,
+    rw ←eq at ph₁,
+    admit,
+    -- induction φ,
+    
+    -- simp at ph₁,
+
+    
+end
+
+section semantics
+
+parameters {α : Type u} [inhabited α]
+
+-- functional interpretation
+def fint  {n : ℕ} := nary n → (fin n → α) → α
+-- relational interpretation
+def rint {n : ℕ} := nrary n → (fin n → α) → Prop
+-- variable assignment
+def vasgn := ℕ → α
+
+parameter exists_ass : nonempty vasgn
+
+structure model :=
+    (I₁ : Π {n}, @fint n)
+    -- required because any constant that would map
+    -- to the default value, would be a "generic point"
+    -- of the type α, i.e. any of its properties would be
+    -- true of any instance of α.
+    (constant_no_default : ∀ f : nary 0, I₁ f fin_zero_elim ≠ default α)
+    (I₂ : Π {n}, @rint n)
+
+-- @[reducible]
+def model.reference' (M : model) : term → vasgn → α
+| (term.var x) asg := asg x
+| (@term.app _ _ _ _ _ _ _ 0 f _) _ := model.I₁ M f fin_zero_elim
+| (@term.app _ _ _ _ _ _ _ (n+1) f v) asg := let v₂ := λ k, model.reference' (v k) asg
+                                             in model.I₁ M f v₂
+-- An unavoidable trick.
+-- It is just ridiculously hard to try any other
+-- alternative. I gained A LOT of productivity
+-- from this.
+| _ _ := default α
+
+-- If the default value is considered to be
+-- a non-existent reference, like an option.none,
+-- then this reference is only defined for pterms.
+def model.reference (M : model) : pterm → α
+| ⟨(@term.app _ _ _ _ _ _ _ 0 f _),_⟩ := model.I₁ M f fin_zero_elim
+| ⟨(@term.app _ _ _ _ _ _ _ (n+1) f v),p⟩ := let v₂ := λ k, model.reference ⟨v k,
+                                            begin
+                                                admit,
+                                            end⟩
+                                             in model.I₁ M f v₂
+| _ := sorry
+-- | t := M.reference' t.val (λx, default α)
+using_well_founded well_founded_tactics.default
+-- begin
+--     constructor,
+--     intros x y,
+--     exact `[exact well_founded_tactics.cancel_nat_add_lt],
+--     exact assumption,
+-- end
+
+
+def model.satisfies' : model → uformula → vasgn → Prop
+| M (uformula.relational r v) asg := 
+          M.I₂ r $ λm,  M.reference' (v m) asg
+| M (uformula.equation t₁ t₂) asg :=
+    let x := model.reference' M t₁ asg,
+        y := model.reference' M t₂ asg
+    in x = y
+| M uformula.true _ := true
+| M uformula.false _ := false
+| M (uformula.for_all x φ) asg :=
+    ∀ (a : α) (ass : vasgn),
+    ass x = a →
+    (∀ y, y ≠ x → ass y = asg y) →
+    M.satisfies' φ ass
+| M (uformula.exist x φ) asg :=
+    ∃ (a : α),
+    ∀ (ass : vasgn),
+    ass x = a →
+    (∀ y, y ≠ x → ass y = asg y) →
+    M.satisfies' φ ass
+| M (uformula.and φ ψ) asg :=
+    let x := model.satisfies' M φ asg,
+        y := model.satisfies' M ψ asg
+    in x ∧ y
+| M (uformula.or φ ψ) asg := 
+    let x := model.satisfies' M φ asg,
+        y := model.satisfies' M ψ asg
+    in x ∨ y
+| M (uformula.if_then φ ψ) asg :=
+    let x := model.satisfies' M φ asg,
+        y := model.satisfies' M ψ asg
+    in x → y
+
+
+@[reducible]
+def model.satisfies : model → uformula → Prop
+| M φ := ∀ (ass : vasgn), M.satisfies' φ ass
+
+local infixr `⊨₁`:55 := model.satisfies
+local infixr `⊢`:55 := minimal.entails
+
+include exists_ass
+lemma false_is_unsat : ¬∃ M : model, M ⊨₁ uformula.false :=
+begin
+    intro h,
+    obtain ⟨M, h⟩ := h,
+    tactic.unfreeze_local_instances,
+    obtain ⟨x⟩ := exists_ass,
+    exact h x,
+end
+omit exists_ass
+
+def model.for : model → set uformula → Prop
+| M Γ := ∀ φ ∈ Γ, M ⊨₁ φ
+
+-- semantic consequence
+-- remember Γ and φ are already defined
+def theory.follows : Prop :=
+    ∀ (M : model) ass, (∀ ψ ∈ Γ, M.satisfies' ψ ass) → M.satisfies' φ ass
+
+local infixr `⊨`:55 := theory.follows
+
+
+def vasgn.bind (ass : vasgn) (x : ℕ) (val : α) : vasgn :=
+    λy, if y = x then val else ass y
+
+-- lemma uformula.rw.semantics (φ : uformula) 
+--                             (x : ℕ)
+--                             (h₀ : x ∈ φ.free)
+--                             (ass : vasgn)
+--                             (M : model)
+--                             (t : pterm)
+--                             : 
+--                             M.satisfies' φ ass →
+--                             M.satisfies' (φ.rw x t.val)
+--                             (ass.bind x (M.reference' t.val ass))
+--                             :=
+-- begin
+--     -- intro h,
+--     induction φ;
+--     dunfold uformula.rw; try{simp};
+--     dunfold model.satisfies';
+--     intro h,
+--     -- have c₁ : (λ (m : fin φ_n), M.reference' (φ_v m) ass) = (flip M.reference' ass) ∘ φ_v,
+--     --     dsimp [flip, function.comp],
+--     --     refl,
+--     have c : ∀ m, (M.reference' ((φ_v m).rw x t.val) (ass.bind x (M.reference' t.val ass))) = M.reference' (φ_v m) ass,
+--         focus {
+--             intro m,
+--             induction (φ_v m);
+--             dunfold term.rw;
+--             dunfold vasgn.bind,
+--             dunfold model.reference',
+--             by_cases h₂ : x = a;
+--                 simp [h₂],
+--                 obtain ⟨t, pt₁, pt₂⟩ := t,
+--                 induction t,
+--                     dunfold model.reference',
+--                     simp,
+                
+--                 revert pt₁,
+--                 dunfold term.denotes,
+--                 dunfold term.vars,
+--                 simp,
+--                     revert pt₂,
+--                     dunfold term.concrete,
+--                     contradiction,
+--                 simp,
+--                 induction t_n;
+--                 dunfold model.reference',
+                
+--                     -- dunfold model.reference',
+
+--         }
+
+            
+
+-- end
+
+-- So pretty.
+theorem soundness : Γ ⊢ φ → Γ ⊨ φ :=
+begin
+    intros entails M ass h,
+    induction entails,
+    -- case reflexive
+    exact h entails_φ entails_h,
+    -- case transitivity
+    apply entails_ih_h₂,
+    intros ψ H,
+    exact entails_ih_h₁ ψ H h,
+    -- case and.intro
+    have c₁ := entails_ih_h₁ h,
+    have c₂ := entails_ih_h₂ h,
+    exact ⟨c₁, c₂⟩,
+    -- case and.elim_left
+    have sat := entails_ih h,
+    revert sat,
+    dunfold model.satisfies',
+    simp,
+    intros sat aux,
+    exact sat,
+    -- case and.elim_right
+    have sat := entails_ih h,
+    revert sat,
+    repeat {dunfold model.satisfies', simp},
+    left,
+    exact entails_ih h,
+    right,
+    exact entails_ih h,
+    -- case or_intro_left
+    -- already solved
+    -- case or_intro_right
+    -- already solved
+    -- case or_elim
+    have c₁ := entails_ih_h₁ h,
+    have c₂ := entails_ih_h₂ h,
+    have c₃ := entails_ih_h₃ h,
+    tactic.unfreeze_local_instances,
+    dunfold model.satisfies' at *,
+    simp at *,
+    cases c₁,
+        exact c₂ c₁,
+    exact c₃ c₁,
+    -- case modus ponens
+    have c₁ := entails_ih_h₁ h,
+    have c₂ := entails_ih_h₂ h,
+    revert c₁,
+    dunfold model.satisfies',
+    simp,
+    intro c₁,
+    exact c₁ c₂,
+    -- case intro
+    intro h₂,
+    have sat := entails_ih,
+    apply sat,
+    intros ψ H,
+    cases H,
+    exact h ψ H,
+    simp at H,
+    rwa H,
+    -- case true.intro
+    trivial,
+    -- case universal intro
+    -- intros x asg h₁ h₂,
+    -- have sat := entails_ih h,
+    -- focus {
+    --     induction entails_φ;
+    --     revert sat;
+    --     dunfold uformula.rw;
+    --     dunfold model.satisfies';
+    --     try{dunfold flip};
+    --     try{dunfold vector.of_fn};
+    --     try{dunfold vector.map},
+    --         intro sat,
+    -- },
+    admit,
+    -- case universal elim
+    -- focus {
+    --     induction entails_φ;
+    --     have sat := entails_ih h;
+    --     revert sat;
+    --     dunfold uformula.rw; try{simp},
+    --     -- I cant go any further applying strategies to
+    --     -- all goals because the linter gets very slow.
+    --     dunfold model.satisfies', try{simp},
+    --         intro sat,
+    -- },
+    admit,
+    -- case exists intro
+    have sat := entails_ih h,
+    existsi M.reference' entails_t ass,
+    intros asg h₁ h₂,
+    admit,
+    -- case exists elim
+    admit,
+    -- case identity intro
+    -- already solved
+    -- case identity elim
+    admit,
+end
+
+
+
+end semantics
+
+section consistency
+end consistency
+
+end formulas
+end logic
