src/nec_being.lean
@@ -1,0 +1,69 @@
+import tactic.tidy
+
+universe u
+
+section necessary
+
+parameter entity : Type u
+parameter situation : Type u
+parameter exist : entity → Prop
+parameter obtain : situation → Prop
+parameter cause : entity → situation → Prop
+parameter necessary : Prop → Prop
+
+def possible (p : Prop) := ¬ necessary (¬ p)
+
+local notation `⋄` := possible
+local notation `□` := necessary
+
+def necessary (e : entity) := □ (exist e)
+
+-- #check ∃ e, ⋄ (necessary e)
+
+def contingent₁ (e : entity) := 
+    ¬ □ (exist e) ∧ ⋄ (exist e)
+
+def contingent₂ (s : situation) := 
+    ¬ □ (obtain s) ∧ ⋄ (obtain s)
+
+def has_causal_powers (e : entity) :=
+    ∃ s, ⋄ (cause e s)
+
+def causable (s : situation) :=
+    ∃ e, ⋄ (cause e s)
+
+def necessary_being (e : entity) :=
+    necessary e ∧ has_causal_powers e
+
+def something_uncausable := 
+    (∃ s, contingent₂ s ∧ obtain s) →
+    (∃ s, contingent₂ s ∧ obtain s ∧ ¬ causable s)
+
+parameter h₁ : ¬ □ something_uncausable
+
+include h₁
+lemma c₁ : ⋄ ¬ something_uncausable :=
+    by simp [possible, classical.not_not]; exact h₁
+
+-- lemma c₂ : ¬ something_uncausable →
+--           ∀ s, contingent₂ s →
+--           obtain s →
+--           causable s :=
+-- begin
+--     intros h s con obt,
+-- end
+
+
+
+
+-- theorem God : 
+-- ∃ (w : world) g : entity,
+--  (necessary g)  ∧ (has_causal_powers g) :=
+
+
+
+-- sorry
+
+
+
+end necessary
