src/prop_sat.lean
@@ -1,0 +1,212 @@
+import tactic.tidy tactic.library_search
+
+
+inductive proposition
+| false : proposition
+| true : proposition
+| atomic : ℕ → proposition
+-- | and : proposition → proposition → proposition
+| or : proposition → proposition → proposition
+| not : proposition → proposition
+-- | if_then : proposition → proposition → proposition
+
+-- def proposition.if_then : proposition → proposition → proposition
+-- | φ ψ := proposition.or (proposition.not φ) ψ
+
+-- notation p `⇒` q := proposition.if_then p q
+
+-- def proposition.not :  proposition → proposition := λ p, p ⇒ proposition.false
+
+def proposition.and : proposition → proposition → proposition
+| φ ψ := proposition.not $ proposition.or (proposition.not φ) (proposition.not ψ)
+
+-- def proposition.iff : proposition → proposition → proposition
+-- | φ ψ := proposition.and (φ ⇒ ψ) (ψ ⇒ φ) 
+
+def proposition.eval : proposition → (ℕ → bool) → bool
+| proposition.false _ := ff
+| proposition.true _ := tt
+| (proposition.atomic n) f := if f n then tt else ff
+-- | (proposition.and φ ψ) f := φ.eval f && ψ.eval f  
+| (proposition.or φ ψ) f := φ.eval f || ψ.eval f
+| (proposition.not φ) f := not (φ.eval f)
+-- | (proposition.if_then φ ψ) f := not (φ.eval f) || ψ.eval f
+
+def proposition.appears : proposition → ℕ → bool
+| proposition.false _ := ff
+| proposition.true  _ := ff
+| (proposition.atomic m) n := if n = m then tt else ff
+-- | (proposition.and φ ψ) n := φ.appears n || ψ.appears n
+| (proposition.or φ ψ) n := φ.appears n || ψ.appears n
+| (proposition.not φ) f := φ.appears f
+-- | (proposition.if_then φ ψ) n := φ.appears n || ψ.appears n
+
+def theory.appears : list proposition → ℕ → bool
+| [] _ :=  ff
+| (x::xs) n := x.appears n || theory.appears xs n
+
+lemma theory.exists : ∀ (Γ : list proposition) n, 
+                      theory.appears Γ n →
+                      ∃ φ ∈ Γ, proposition.appears φ n
+                      :=
+begin
+    intros Γ n h,
+    induction Γ;
+        simp [theory.appears] at h,
+        contradiction,
+    cases h,
+        existsi Γ_hd,
+        fsplit, simp,
+        assumption,
+    obtain ⟨φ, c₁, c₂⟩ := Γ_ih h,
+    existsi φ,
+    fsplit,
+        simp [c₁],
+    assumption,
+end
+
+def proposition.satisfiable (φ : proposition) :=
+    ∃ I : ℕ → bool, φ.eval I 
+
+
+-- This code here actually implements the sat solver...
+-- FROM A TACTIC PROOF!!!
+instance sat_solver (φ : proposition) : decidable φ.satisfiable :=
+let I₁ := λn : ℕ, tt in
+begin
+    induction φ,
+    -- case false
+        left,
+        intro h,
+        obtain ⟨I, c⟩ := h,
+        simp [proposition.eval] at c,
+        contradiction,
+    -- case true
+        right,
+        existsi I₁,
+        simp [proposition.eval],
+    -- case atomic
+        right,
+        existsi I₁,
+        simp [proposition.eval],
+    -- case and
+        -- This is actually hard.
+        -- We only managed to prove that if
+        -- either side of the conjunction is
+        -- unsat, then the conjunction is unsat.
+        -- maybe that is why most algorithms assume
+        -- that the proposition is on
+        -- a particular normal form.
+        -- So when we got to this point,
+        -- we changed the definition of proposition
+        -- to use only ∨ and ¬, which is 
+        -- functionally complete.
+
+        -- cases φ_ih_a,
+        --     left,
+        --     intro h,
+        --     obtain ⟨I, c⟩ := h,
+        --     simp [proposition.eval] at c,
+        --     replace c : φ_a.satisfiable := ⟨I,c.1⟩,
+        --     contradiction,
+        -- cases φ_ih_a_1,
+        --     left,
+        --     intro h,
+        --     obtain ⟨I, c⟩ := h,
+        --     simp [proposition.eval] at c,
+        --     replace c : φ_a_1.satisfiable := ⟨I,c.2⟩,
+        --     contradiction,
+    -- case or
+        cases φ_ih_a,
+            cases φ_ih_a_1,
+                left,
+                intro h,
+                obtain ⟨I, c⟩ := h,
+                simp [proposition.eval] at c,
+                cases c,
+                    replace c : φ_a.satisfiable := ⟨I,c⟩,
+                    contradiction,
+                replace c : φ_a_1.satisfiable := ⟨I,c⟩,
+                contradiction,
+            right,
+            obtain ⟨I, c⟩ := φ_ih_a_1,
+            existsi I,
+            simp [proposition.eval],
+            right,
+            assumption,
+        right,
+        obtain ⟨I, c⟩ := φ_ih_a,
+        existsi I,
+        simp [proposition.eval],
+        left,
+        assumption,
+    -- case not
+        cases φ_ih,
+            right,
+            have c := not_exists.mp φ_ih I₁,
+            existsi I₁,
+            simp [proposition.eval],
+            simp at c,
+            rw c,
+            simp,
+        admit,
+    -- case if_then
+    -- cases φ_ih_a,
+    --     right,
+    --     existsi I₁,
+    --     simp [proposition.eval],
+    --     have c := not_exists.mp φ_ih_a I₁,
+    --     simp at c,
+    --     left,
+    --     rw c,
+    --     simp,
+    -- cases φ_ih_a_1,
+    --     left,
+    --     intro h,
+    --     obtain ⟨I, c⟩ := h,
+    --     simp [proposition.eval] at c,
+end
+
+def proposition.sat : proposition → bool
+| φ := if φ.satisfiable then tt else ff
+
+#reduce proposition.false.sat
+#reduce proposition.true.sat
+#reduce λ n, (proposition.atomic n).sat
+#reduce λ n, (proposition.or (proposition.atomic n) proposition.false).sat
+#reduce λ n, (proposition.or (proposition.atomic n) (proposition.not $ proposition.atomic n)).sat
+-- #reduce λ n, (proposition.and (proposition.atomic n) (proposition.not $ proposition.atomic n)).sat
+
+def proposition.follows (Γ : list proposition) : proposition → Prop
+| φ :=    ∀ (I : ℕ → bool), 
+          (∀ ψ ∈ Γ, proposition.eval ψ I == tt) →
+          φ.eval I == tt
+
+-- instance proposition_decidable (Γ : list proposition) (φ : proposition) :decidable (φ.follows Γ) :=
+-- begin
+--     induction φ,
+--         admit,
+--     right,
+--     intros I h,
+--     refl,
+--     by_cases (theory.appears Γ φ) = tt,
+--         have c : Prop,
+--             obtain ⟨ψ, c₀, c₁⟩ := theory.exists Γ φ h,
+--         replace h₂ := h₂ ψ c₀,
+--         right,
+--         intros I h₂,
+--         dsimp [proposition.eval],
+--         simp,
+--         -- let ψ := proposition.atomic φ,
+
+--         -- induction Γ;
+--         --     simp [theory.appears] at h,
+--         --     contradiction,
+        
+--         -- have c := h ψ h₂,
+
+-- end
+
+-- def proposition.decide : proposition → set proposition → bool
+-- | φ Γ := if φ.follows Γ then tt else ff
+
