src/tactics.lean
@@ -1,0 +1,34 @@
+import tactic init.meta.interactive_base
+
+open tactic interactive interactive.types
+#check tactic.induction
+#check interactive.induction
+#check mk_const
+#check ``(1)
+#check intro
+#check exact
+
+#check applyc
+#check prod.fst
+#check first
+#check focus
+#check try
+
+meta def tactic.my_tac (e : expr) : tactic unit :=
+    do cases ← induction e,
+    focus (list.map (λx, try $ applyc (prod.fst x)) cases)
+
+meta def my_tac (q : parse texpr) : tactic unit :=
+    i_to_expr ``(%%q) >>= tactic.my_tac
+
+inductive test
+| a : test
+| b : test
+
+example : ∀ t : test, ∃ x, x = t := 
+begin
+    intro t,
+    have h := true.intro,
+    -- my_tac h,
+    admit
+end
